refactor BetreeSpec around the new BetreeStep type
each step has: (i) a validation function (ii) a function to return a list of ops
and (iii) a function to return a list of reads

disk-betree/BetreeSpec.dfy
@@ -3,7 +3,6 @@ include "../lib/sequences.dfy"
 include "../lib/Maps.dfy"
 include "MapSpec.dfy"
 include "Graph.dfy"
-include "BlockCache.dfy"
 
 module BetreeGraph refines Graph {
   import MS = MapSpec
@@ -25,8 +24,7 @@ module BetreeBlockInterface refines BlockInterface {
   import G = BetreeGraph
 }
 
-module BetreeSpecCommon {
-
+module BetreeSpec {
   import MS = MapSpec
   import opened G = BetreeGraph
   import opened Sequences
@@ -47,7 +45,8 @@ module BetreeSpecCommon {
   }
 
   // Now we define the state machine
-  
+
+  //// Insert
 
   function EmptyNode() : Node {
     var buffer := imap key | MS.InDomain(key) :: [Insertion(MS.EmptyValue())];
@@ -66,6 +65,93 @@ module BetreeSpecCommon {
     Node(node.children, AddMessageToBuffer(node.buffer, key, msg))
   }
 
+  datatype MessageInsertion = MessageInsertion(key: Key, msg: BufferEntry, oldroot: Node)
+
+  predicate ValidInsertion(ins: MessageInsertion) {
+    && WFNode(ins.oldroot)
+  }
+
+  function InsertionReads(ins: MessageInsertion): seq<ReadOp>
+  requires ValidInsertion(ins)
+  {
+    [G.ReadOp(Root(), ins.oldroot)]
+  }
+
+  function InsertionOps(ins: MessageInsertion) : seq<Op>
+  requires ValidInsertion(ins)
+  {
+    var newroot := AddMessageToNode(ins.oldroot, ins.key, ins.msg);
+    var writeop := G.WriteOp(Root(), newroot);
+    [writeop]
+  }
+
+  //// Flush
+
+  datatype NodeFlush = NodeFlush(parentref: Reference, parent: Node, childref: Reference, child: Node, newchildref: Reference)
+
+  predicate ValidFlush(flush: NodeFlush)
+  {
+    && WFNode(flush.parent)
+    && WFNode(flush.child)
+  }
+
+  function FlushReads(flush: NodeFlush) : seq<ReadOp>
+  requires ValidFlush(flush)
+  {
+    [
+      G.ReadOp(flush.parentref, flush.parent),
+      G.ReadOp(flush.childref, flush.child)
+    ]
+  }
+
+  function FlushOps(flush: NodeFlush) : seq<Op>
+  requires ValidFlush(flush)
+  {
+    // TODO move all this junk into the NodeFlush object
+    var parentref := flush.parentref;
+    var parent := flush.parent;
+    var childref := flush.childref;
+    var child := flush.child;
+    var newchildref := flush.newchildref;
+    var movedKeys := iset k | k in parent.children && parent.children[k] == childref;
+    var newbuffer := imap k :: (if k in movedKeys then parent.buffer[k] + child.buffer[k] else child.buffer[k]);
+    var newchild := Node(child.children, newbuffer);
+    var newparentbuffer := imap k :: (if k in movedKeys then [] else parent.buffer[k]);
+    var newparentchildren := imap k | k in parent.children :: (if k in movedKeys then newchildref else parent.children[k]);
+    var newparent := Node(newparentchildren, newparentbuffer);
+    var allocop := G.AllocOp(newchildref, newchild);
+    var writeop := G.WriteOp(parentref, newparent);
+    [allocop, writeop]
+  }
+
+  //// Grow
+
+  datatype RootGrowth = RootGrowth(oldroot: Node, newchildref: Reference)
+
+  predicate ValidGrow(growth: RootGrowth)
+  {
+    true
+  }
+
+  function GrowReads(growth: RootGrowth) : seq<ReadOp>
+  requires ValidGrow(growth)
+  {
+    [G.ReadOp(Root(), growth.oldroot)]
+  }
+
+  function GrowOps(growth: RootGrowth) : seq<Op>
+  requires ValidGrow(growth)
+  {
+    var newroot := Node(
+        imap key | MS.InDomain(key) :: growth.newchildref,
+        imap key | MS.InDomain(key) :: []);
+    var allocop := G.AllocOp(growth.newchildref, growth.oldroot);
+    var writeop := G.WriteOp(Root(), newroot);
+    [allocop, writeop]
+  }
+
+  //// Split
+
   datatype NodeFusion = NodeFusion(
     parentref: Reference,
     fused_childref: Reference,
@@ -80,45 +166,6 @@ module BetreeSpecCommon {
     left_keys: iset<Key>,
     right_keys: iset<Key>
   )
-}
-
-module BetreeSpec refines BetreeSpecCommon {
-  import Tr = BetreeBlockInterface
-
-  predicate InsertMessage(k: Tr.Constants, s: Tr.Variables, s': Tr.Variables, key: Key, msg: BufferEntry, oldroot: Node) {
-    && Tr.Reads(k, s, Root(), oldroot)
-    && WFNode(oldroot)
-    && var newroot := AddMessageToNode(oldroot, key, msg);
-    && var writeop := G.WriteOp(Root(), newroot);
-    && Tr.OpTransaction(k, s, s', [writeop])
-  }
-
-  predicate Flush(k: Tr.Constants, s: Tr.Variables, s': Tr.Variables, parentref: Reference, parent: Node, childref: Reference, child: Node, newchildref: Reference) {
-    var movedKeys := iset k | k in parent.children && parent.children[k] == childref;
-    && Tr.Reads(k, s, parentref, parent)
-    && Tr.Reads(k, s, childref, child)
-    && WFNode(parent)
-    && WFNode(child)
-    && var newbuffer := imap k :: (if k in movedKeys then parent.buffer[k] + child.buffer[k] else child.buffer[k]);
-    && var newchild := Node(child.children, newbuffer);
-    && var newparentbuffer := imap k :: (if k in movedKeys then [] else parent.buffer[k]);
-    && var newparentchildren := imap k | k in parent.children :: (if k in movedKeys then newchildref else parent.children[k]);
-    && var newparent := Node(newparentchildren, newparentbuffer);
-    && var allocop := G.AllocOp(newchildref, newchild);
-    && var writeop := G.WriteOp(parentref, newparent);
-    && Tr.OpTransaction(k, s, s', [allocop, writeop])
-  }
-
-  predicate Grow(k: Tr.Constants, s: Tr.Variables, s': Tr.Variables, oldroot: Node, newchildref: Reference) {
-    && Tr.Reads(k, s, Root(), oldroot)
-    && var newchild := oldroot;
-    && var newroot := Node(
-        imap key | MS.InDomain(key) :: newchildref,
-        imap key | MS.InDomain(key) :: []);
-    && var allocop := G.AllocOp(newchildref, newchild);
-    && var writeop := G.WriteOp(Root(), newroot);
-    && Tr.OpTransaction(k, s, s', [allocop, writeop])
-  }
 
   predicate ValidFusion(fusion: NodeFusion)
   {
@@ -141,119 +188,101 @@ module BetreeSpec refines BetreeSpecCommon {
     && (forall key :: key in fusion.right_keys ==> IMapsAgreeOnKey(fusion.fused_child.buffer, fusion.right_child.buffer, key))
   }
 
-  predicate Split(k: Tr.Constants, s: Tr.Variables, s': Tr.Variables, fusion: NodeFusion)
+  predicate ValidSplit(fusion: NodeFusion)
   {
-    && Tr.Reads(k, s, fusion.parentref, fusion.fused_parent)
-    && Tr.Reads(k, s, fusion.fused_childref, fusion.fused_child)
-    && ValidFusion(fusion)
     && WFNode(fusion.fused_parent)
     && WFNode(fusion.fused_child)
     && WFNode(fusion.left_child)
     && WFNode(fusion.right_child)
-    && var allocop_left := G.AllocOp(fusion.left_childref, fusion.left_child);
-    && var allocop_right := G.AllocOp(fusion.right_childref, fusion.right_child);
-    && var writeop := G.WriteOp(fusion.parentref, fusion.split_parent);
-    && Tr.OpTransaction(k, s, s', [allocop_left, allocop_right, writeop])
-  }
-
-  predicate Merge(k: Tr.Constants, s: Tr.Variables, s': Tr.Variables, fusion: NodeFusion)
-  {
-    && Tr.Reads(k, s, fusion.parentref, fusion.split_parent)
-    && Tr.Reads(k, s, fusion.left_childref, fusion.left_child)
-    && Tr.Reads(k, s, fusion.right_childref, fusion.right_child)
     && ValidFusion(fusion)
-    && var allocop := G.AllocOp(fusion.fused_childref, fusion.fused_child);
-    && var writeop := G.WriteOp(fusion.parentref, fusion.fused_parent);
-    && Tr.OpTransaction(k, s, s', [allocop, writeop])
-  }
-}
-
-module BetreeGraphBlockCache refines BlockCache {
-  import G = BetreeGraph
-}
-
-module BetreeSpecForBlockCache refines BetreeSpecCommon {
-  import Tr = BetreeGraphBlockCache
-
-  predicate InsertMessage(k: Tr.Constants, s: Tr.Variables, s': Tr.Variables, key: Key, msg: BufferEntry, oldroot: Node) {
-    && Tr.Reads(k, s, Root(), oldroot)
-    && WFNode(oldroot)
-    && var newroot := AddMessageToNode(oldroot, key, msg);
-    && var writeop := G.WriteOp(Root(), newroot);
-    && Tr.OpTransaction(k, s, s', [writeop])
   }
 
-  predicate Flush(k: Tr.Constants, s: Tr.Variables, s': Tr.Variables, parentref: Reference, parent: Node, childref: Reference, child: Node, newchildref: Reference) {
-    var movedKeys := iset k | k in parent.children && parent.children[k] == childref;
-    && Tr.Reads(k, s, parentref, parent)
-    && Tr.Reads(k, s, childref, child)
-    && WFNode(parent)
-    && WFNode(child)
-    && var newbuffer := imap k :: (if k in movedKeys then parent.buffer[k] + child.buffer[k] else child.buffer[k]);
-    && var newchild := Node(child.children, newbuffer);
-    && var newparentbuffer := imap k :: (if k in movedKeys then [] else parent.buffer[k]);
-    && var newparentchildren := imap k | k in parent.children :: (if k in movedKeys then newchildref else parent.children[k]);
-    && var newparent := Node(newparentchildren, newparentbuffer);
-    && var allocop := G.AllocOp(newchildref, newchild);
-    && var writeop := G.WriteOp(parentref, newparent);
-    && Tr.OpTransaction(k, s, s', [allocop, writeop])
-  }
-
-  predicate Grow(k: Tr.Constants, s: Tr.Variables, s': Tr.Variables, oldroot: Node, newchildref: Reference) {
-    && Tr.Reads(k, s, Root(), oldroot)
-    && var newchild := oldroot;
-    && var newroot := Node(
-        imap key | MS.InDomain(key) :: newchildref,
-        imap key | MS.InDomain(key) :: []);
-    && var allocop := G.AllocOp(newchildref, newchild);
-    && var writeop := G.WriteOp(Root(), newroot);
-    && Tr.OpTransaction(k, s, s', [allocop, writeop])
-  }
-
-  predicate ValidFusion(fusion: NodeFusion)
+  function SplitReads(fusion: NodeFusion) : seq<ReadOp>
+  requires ValidSplit(fusion)
   {
-    && fusion.left_keys !! fusion.right_keys
-    && (forall key :: key in fusion.left_keys ==> IMapsTo(fusion.fused_parent.children, key, fusion.fused_childref))
-    && (forall key :: key in fusion.left_keys ==> IMapsTo(fusion.split_parent.children, key, fusion.left_childref))
-
-    && (forall key :: key in fusion.right_keys ==> IMapsTo(fusion.fused_parent.children, key, fusion.fused_childref))
-    && (forall key :: key in fusion.right_keys ==> IMapsTo(fusion.split_parent.children, key, fusion.right_childref))
-
-    && (forall key :: (key !in fusion.left_keys) && (key !in fusion.right_keys) ==>
-      IMapsAgreeOnKey(fusion.split_parent.children, fusion.fused_parent.children, key))
-
-    && fusion.fused_parent.buffer == fusion.split_parent.buffer
-
-    && (forall key :: key in fusion.left_keys ==> IMapsAgreeOnKey(fusion.fused_child.children, fusion.left_child.children, key))
-    && (forall key :: key in fusion.left_keys ==> IMapsAgreeOnKey(fusion.fused_child.buffer, fusion.left_child.buffer, key))
-
-    && (forall key :: key in fusion.right_keys ==> IMapsAgreeOnKey(fusion.fused_child.children, fusion.right_child.children, key))
-    && (forall key :: key in fusion.right_keys ==> IMapsAgreeOnKey(fusion.fused_child.buffer, fusion.right_child.buffer, key))
+    [
+      ReadOp(fusion.parentref, fusion.fused_parent),
+      ReadOp(fusion.fused_childref, fusion.fused_child)
+    ]
   }
 
-  predicate Split(k: Tr.Constants, s: Tr.Variables, s': Tr.Variables, fusion: NodeFusion)
+  function SplitOps(fusion: NodeFusion) : seq<Op>
+  requires ValidSplit(fusion)
   {
-    && Tr.Reads(k, s, fusion.parentref, fusion.fused_parent)
-    && Tr.Reads(k, s, fusion.fused_childref, fusion.fused_child)
-    && ValidFusion(fusion)
-    && WFNode(fusion.fused_parent)
-    && WFNode(fusion.fused_child)
-    && WFNode(fusion.left_child)
-    && WFNode(fusion.right_child)
-    && var allocop_left := G.AllocOp(fusion.left_childref, fusion.left_child);
-    && var allocop_right := G.AllocOp(fusion.right_childref, fusion.right_child);
-    && var writeop := G.WriteOp(fusion.parentref, fusion.split_parent);
-    && Tr.OpTransaction(k, s, s', [allocop_left, allocop_right, writeop])
+    [
+      G.AllocOp(fusion.left_childref, fusion.left_child),
+      G.AllocOp(fusion.right_childref, fusion.right_child),
+      G.WriteOp(fusion.parentref, fusion.split_parent)
+    ]
   }
 
-  predicate Merge(k: Tr.Constants, s: Tr.Variables, s': Tr.Variables, fusion: NodeFusion)
+  //// Merge
+
+  predicate ValidMerge(fusion: NodeFusion)
   {
-    && Tr.Reads(k, s, fusion.parentref, fusion.split_parent)
-    && Tr.Reads(k, s, fusion.left_childref, fusion.left_child)
-    && Tr.Reads(k, s, fusion.right_childref, fusion.right_child)
-    && ValidFusion(fusion)
-    && var allocop := G.AllocOp(fusion.fused_childref, fusion.fused_child);
-    && var writeop := G.WriteOp(fusion.parentref, fusion.fused_parent);
-    && Tr.OpTransaction(k, s, s', [allocop, writeop])
+    ValidFusion(fusion)
+  }
+
+  function MergeReads(fusion: NodeFusion) : seq<ReadOp>
+  requires ValidMerge(fusion)
+  {
+    [
+      ReadOp(fusion.parentref, fusion.split_parent),
+      ReadOp(fusion.left_childref, fusion.left_child),
+      ReadOp(fusion.right_childref, fusion.right_child)
+    ]
+  }
+
+  function MergeOps(fusion: NodeFusion) : seq<Op>
+  requires ValidMerge(fusion)
+  {
+    [
+      G.AllocOp(fusion.fused_childref, fusion.fused_child),
+      G.WriteOp(fusion.parentref, fusion.fused_parent)
+    ]
+  }
+
+  //// All together
+
+  datatype BetreeStep =
+    | BetreeInsert(ins: MessageInsertion)
+    | BetreeFlush(flush: NodeFlush)
+    | BetreeGrow(growth: RootGrowth)
+    | BetreeSplit(fusion: NodeFusion)
+    | BetreeMerge(fusion: NodeFusion)
+
+  predicate ValidBetreeStep(step: BetreeStep)
+  {
+    match step {
+      case BetreeInsert(ins) => ValidInsertion(ins)
+      case BetreeFlush(flush) => ValidFlush(flush)
+      case BetreeGrow(growth) => ValidGrow(growth)
+      case BetreeSplit(fusion) => ValidSplit(fusion)
+      case BetreeMerge(fusion) => ValidMerge(fusion)
+    }
+  }
+
+  function BetreeStepReads(step: BetreeStep) : seq<ReadOp>
+  requires ValidBetreeStep(step)
+  {
+    match step {
+      case BetreeInsert(ins) => InsertionReads(ins)
+      case BetreeFlush(flush) => FlushReads(flush)
+      case BetreeGrow(growth) => GrowReads(growth)
+      case BetreeSplit(fusion) => SplitReads(fusion)
+      case BetreeMerge(fusion) => MergeReads(fusion)
+    }
+  }
+
+  function BetreeStepOps(step: BetreeStep) : seq<Op>
+  requires ValidBetreeStep(step)
+  {
+    match step {
+      case BetreeInsert(ins) => InsertionOps(ins)
+      case BetreeFlush(flush) => FlushOps(flush)
+      case BetreeGrow(growth) => GrowOps(growth)
+      case BetreeSplit(fusion) => SplitOps(fusion)
+      case BetreeMerge(fusion) => MergeOps(fusion)
+    }
   }
 }
